<?xml version="1.0" encoding="UTF-8"?>
<rdf:RDF xmlns:dcterms="http://purl.org/dc/terms/" xmlns:foaf="http://xmlns.com/foaf/0.1/"
         xmlns:office="urn:oasis:names:tc:opendocument:xmlns:office:1.0"
         xmlns:text="urn:oasis:names:tc:opendocument:xmlns:text:1.0"
         xmlns:table="urn:oasis:names:tc:opendocument:xmlns:table:1.0"
         xmlns:rdf="http://www.w3.org/1999/02/22-rdf-syntax-ns#"
         xmlns:rdfs="http://www.w3.org/2000/01/rdf-schema#"
         xmlns:skos="http://www.w3.org/2004/02/skos/core#"
         xmlns:cc="http://creativecommons.org/ns#"
         xmlns:ex="http://example.org/">
   <foaf:Document rdf:about="">
      <cc:attributionName>University of Oxford</cc:attributionName>
      <cc:attributionURL rdf:resource="https://data.ox.ac.uk/doc/ox-rdf/concept-scheme"/>
      <dcterms:license rdf:resource="http://creativecommons.org/publicdomain/zero/1.0/"/>
   </foaf:Document>
   <skos:ConceptScheme rdf:about="https://data.ox.ac.uk/id/ox-rdf/concept-scheme">
      <skos:prefLabel xml:lang="en">Oxford Skills Classification</skos:prefLabel>
      <skos:altLabel>OxSC</skos:altLabel>
      <rdfs:comment>The Oxford Skills Classification is a simple way to categorize skills courses by subject area.</rdfs:comment>
      <cc:attributionName>University of Oxford</cc:attributionName>
      <cc:attributionURL rdf:resource="https://data.ox.ac.uk/doc/ox-rdf/concept-scheme"/>
      <dcterms:license rdf:resource="http://creativecommons.org/publicdomain/zero/1.0/"/>
      <skos:hasTopConcept>
         <skos:Concept rdf:about="https://data.ox.ac.uk/id/ox-rdf/descriptor/RD">
            <skos:prefLabel>General Researcher Development</skos:prefLabel>
            <skos:notation rdf:datatype="https://data.ox.ac.uk/id/ox-rdf/notation">RD</skos:notation>
            <skos:inScheme rdf:resource="https://data.ox.ac.uk/id/ox-rdf/concept-scheme"/>
            <skos:narrower>
               <skos:Concept rdf:about="https://data.ox.ac.uk/id/ox-rdf/descriptor/CO">
                  <skos:prefLabel>Computing</skos:prefLabel>
                  <skos:notation rdf:datatype="https://data.ox.ac.uk/id/ox-rdf/notation">CO</skos:notation>
                  <skos:definition>IT Skills: this might include using software; programming; data manipulation; working with hardware, etc.</skos:definition>
                  <skos:related rdf:resource="https://data.ox.ac.uk/id/ox-rdf/domain/study-and-research-skills"/>
                  <skos:inScheme rdf:resource="https://data.ox.ac.uk/id/ox-rdf/concept-scheme"/>
               </skos:Concept>
            </skos:narrower>
            <skos:narrower>
               <skos:Concept rdf:about="https://data.ox.ac.uk/id/ox-rdf/descriptor/DA">
                  <skos:prefLabel>Data Analysis</skos:prefLabel>
                  <skos:notation rdf:datatype="https://data.ox.ac.uk/id/ox-rdf/notation">DA</skos:notation>
                  <skos:definition>Note that this is about analysing, evaluating, synthesising and critiquing DATA specifically, as opposed to broader analytical skills (see Study and Research Skills)</skos:definition>
                  <skos:related rdf:resource="https://data.ox.ac.uk/id/ox-rdf/domain/study-and-research-skills"/>
                  <skos:inScheme rdf:resource="https://data.ox.ac.uk/id/ox-rdf/concept-scheme"/>
               </skos:Concept>
            </skos:narrower>
            <skos:narrower>
               <skos:Concept rdf:about="https://data.ox.ac.uk/id/ox-rdf/descriptor/DM">
                  <skos:prefLabel>Data Management</skos:prefLabel>
                  <skos:notation rdf:datatype="https://data.ox.ac.uk/id/ox-rdf/notation">DM</skos:notation>
                  <skos:definition>This is all about looking after data (otherwise known as research integrity), whether in theory or by practical application. </skos:definition>
                  <skos:related rdf:resource="https://data.ox.ac.uk/id/ox-rdf/domain/study-and-research-skills"/>
                  <skos:inScheme rdf:resource="https://data.ox.ac.uk/id/ox-rdf/concept-scheme"/>
               </skos:Concept>
            </skos:narrower>
            <skos:narrower>
               <skos:Concept rdf:about="https://data.ox.ac.uk/id/ox-rdf/descriptor/FW">
                  <skos:prefLabel>Field Work</skos:prefLabel>
                  <skos:notation rdf:datatype="https://data.ox.ac.uk/id/ox-rdf/notation">FW</skos:notation>
                  <skos:definition>Been on a productive trip lately?</skos:definition>
                  <skos:related rdf:resource="https://data.ox.ac.uk/id/ox-rdf/domain/study-and-research-skills"/>
                  <skos:inScheme rdf:resource="https://data.ox.ac.uk/id/ox-rdf/concept-scheme"/>
               </skos:Concept>
            </skos:narrower>
            <skos:narrower>
               <skos:Concept rdf:about="https://data.ox.ac.uk/id/ox-rdf/descriptor/IN">
                  <skos:prefLabel>Information skills</skos:prefLabel>
                  <skos:notation rdf:datatype="https://data.ox.ac.uk/id/ox-rdf/notation">IN</skos:notation>
                  <skos:definition>How good are you at seeking out information, and managing it when you find it?</skos:definition>
                  <skos:related rdf:resource="https://data.ox.ac.uk/id/ox-rdf/domain/study-and-research-skills"/>
                  <skos:inScheme rdf:resource="https://data.ox.ac.uk/id/ox-rdf/concept-scheme"/>
               </skos:Concept>
            </skos:narrower>
            <skos:narrower>
               <skos:Concept rdf:about="https://data.ox.ac.uk/id/ox-rdf/descriptor/LS">
                  <skos:prefLabel>Laboratory skills</skos:prefLabel>
                  <skos:notation rdf:datatype="https://data.ox.ac.uk/id/ox-rdf/notation">LS</skos:notation>
                  <skos:definition>How are your skills in the lab, whether that means knowledge or practice?</skos:definition>
                  <skos:related rdf:resource="https://data.ox.ac.uk/id/ox-rdf/domain/study-and-research-skills"/>
                  <skos:inScheme rdf:resource="https://data.ox.ac.uk/id/ox-rdf/concept-scheme"/>
               </skos:Concept>
            </skos:narrower>
            <skos:narrower>
               <skos:Concept rdf:about="https://data.ox.ac.uk/id/ox-rdf/descriptor/LA">
                  <skos:prefLabel>Languages</skos:prefLabel>
                  <skos:notation rdf:datatype="https://data.ox.ac.uk/id/ox-rdf/notation">LA</skos:notation>
                  <skos:definition>If you're learning a new language then record your progress here.</skos:definition>
                  <skos:related rdf:resource="https://data.ox.ac.uk/id/ox-rdf/domain/study-and-research-skills"/>
                  <skos:related rdf:resource="https://data.ox.ac.uk/id/ox-rdf/domain/career-and-personal-development"/>
                  <skos:inScheme rdf:resource="https://data.ox.ac.uk/id/ox-rdf/concept-scheme"/>
               </skos:Concept>
            </skos:narrower>
            <skos:narrower>
               <skos:Concept rdf:about="https://data.ox.ac.uk/id/ox-rdf/descriptor/MM">
                  <skos:prefLabel>Mathematical Methods</skos:prefLabel>
                  <skos:notation rdf:datatype="https://data.ox.ac.uk/id/ox-rdf/notation">MM</skos:notation>
                  <skos:definition>This might include working with numbers, solving problems, understanding different ways of approaching problems mathematically, constructing arguments in numbers, and so on.</skos:definition>
                  <skos:related rdf:resource="https://data.ox.ac.uk/id/ox-rdf/domain/study-and-research-skills"/>
                  <skos:inScheme rdf:resource="https://data.ox.ac.uk/id/ox-rdf/concept-scheme"/>
               </skos:Concept>
            </skos:narrower>
            <skos:narrower>
               <skos:Concept rdf:about="https://data.ox.ac.uk/id/ox-rdf/descriptor/RM">
                  <skos:prefLabel>Research Methods</skos:prefLabel>
                  <skos:notation rdf:datatype="https://data.ox.ac.uk/id/ox-rdf/notation">RM</skos:notation>
                  <skos:definition>Your skills develop in this category as your knowledge of methods grows and you improve the way you apply them.</skos:definition>
                  <skos:related rdf:resource="https://data.ox.ac.uk/id/ox-rdf/domain/study-and-research-skills"/>
                  <skos:inScheme rdf:resource="https://data.ox.ac.uk/id/ox-rdf/concept-scheme"/>
               </skos:Concept>
            </skos:narrower>
            <skos:narrower>
               <skos:Concept rdf:about="https://data.ox.ac.uk/id/ox-rdf/descriptor/ST">
                  <skos:prefLabel>Statistics</skos:prefLabel>
                  <skos:notation rdf:datatype="https://data.ox.ac.uk/id/ox-rdf/notation">ST</skos:notation>
                  <skos:definition>Includes theory and application: your skills improve as your knowledge widens and you get better at applying statistical methods.</skos:definition>
                  <skos:related rdf:resource="https://data.ox.ac.uk/id/ox-rdf/domain/study-and-research-skills"/>
                  <skos:inScheme rdf:resource="https://data.ox.ac.uk/id/ox-rdf/concept-scheme"/>
               </skos:Concept>
            </skos:narrower>
            <skos:narrower>
               <skos:Concept rdf:about="https://data.ox.ac.uk/id/ox-rdf/descriptor/TE">
                  <skos:prefLabel>Technical skills</skos:prefLabel>
                  <skos:notation rdf:datatype="https://data.ox.ac.uk/id/ox-rdf/notation">TE</skos:notation>
                  <skos:definition>Might include, for instance, learning new ways of using research-related gadgets and equipment.</skos:definition>
                  <skos:related rdf:resource="https://data.ox.ac.uk/id/ox-rdf/domain/study-and-research-skills"/>
                  <skos:inScheme rdf:resource="https://data.ox.ac.uk/id/ox-rdf/concept-scheme"/>
               </skos:Concept>
            </skos:narrower>
            <skos:narrower>
               <skos:Concept rdf:about="https://data.ox.ac.uk/id/ox-rdf/descriptor/SR">
                  <skos:prefLabel>Study and Research skills</skos:prefLabel>
                  <skos:notation rdf:datatype="https://data.ox.ac.uk/id/ox-rdf/notation">SR</skos:notation>
                  <skos:definition>Includes, for instance: critical thinking, your ability to evaluate things and solve problems, your techniques and methods for studying and researching a topic.</skos:definition>
                  <skos:related rdf:resource="https://data.ox.ac.uk/id/ox-rdf/domain/study-and-research-skills"/>
                  <skos:inScheme rdf:resource="https://data.ox.ac.uk/id/ox-rdf/concept-scheme"/>
               </skos:Concept>
            </skos:narrower>
            <skos:narrower>
               <skos:Concept rdf:about="https://data.ox.ac.uk/id/ox-rdf/descriptor/CD">
                  <skos:prefLabel>Career Development</skos:prefLabel>
                  <skos:notation rdf:datatype="https://data.ox.ac.uk/id/ox-rdf/notation">CD</skos:notation>
                  <skos:definition>This is about how much you reflect upon and work on developing your career, whether through continual professional development, networking, writing a great CV or through getting better at writing job applications.</skos:definition>
                  <skos:related rdf:resource="https://data.ox.ac.uk/id/ox-rdf/domain/career-and-personal-development"/>
                  <skos:inScheme rdf:resource="https://data.ox.ac.uk/id/ox-rdf/concept-scheme"/>
               </skos:Concept>
            </skos:narrower>
            <skos:narrower>
               <skos:Concept rdf:about="https://data.ox.ac.uk/id/ox-rdf/descriptor/PE">
                  <skos:prefLabel>Personal Effectiveness</skos:prefLabel>
                  <skos:notation rdf:datatype="https://data.ox.ac.uk/id/ox-rdf/notation">PE</skos:notation>
                  <skos:definition>This might include, among many other things: your self-confidence; empathy toward others; sense of responsibility and integrity; time management; ability to balance life and work.</skos:definition>
                  <skos:related rdf:resource="https://data.ox.ac.uk/id/ox-rdf/domain/career-and-personal-development"/>
                  <skos:inScheme rdf:resource="https://data.ox.ac.uk/id/ox-rdf/concept-scheme"/>
               </skos:Concept>
            </skos:narrower>
            <skos:narrower>
               <skos:Concept rdf:about="https://data.ox.ac.uk/id/ox-rdf/descriptor/ET">
                  <skos:prefLabel>Ethics</skos:prefLabel>
                  <skos:notation rdf:datatype="https://data.ox.ac.uk/id/ox-rdf/notation">ET</skos:notation>
                  <skos:definition>How is your knowledge of ethics (related to your research, especially) and how confident are you in applying that knowledge?</skos:definition>
                  <skos:related rdf:resource="https://data.ox.ac.uk/id/ox-rdf/domain/study-and-research-skills"/>
                  <skos:inScheme rdf:resource="https://data.ox.ac.uk/id/ox-rdf/concept-scheme"/>
               </skos:Concept>
            </skos:narrower>
            <skos:narrower>
               <skos:Concept rdf:about="https://data.ox.ac.uk/id/ox-rdf/descriptor/IP">
                  <skos:prefLabel>Intellectual property skills</skos:prefLabel>
                  <skos:notation rdf:datatype="https://data.ox.ac.uk/id/ox-rdf/notation">IP</skos:notation>
                  <skos:definition>These skills include: knowledge of copyright and intellectual property, ethical considerations, respect for the work of others, knowing how to attribute authorship, knowing when to maintain confidentiality, and so on.</skos:definition>
                  <skos:related rdf:resource="https://data.ox.ac.uk/id/ox-rdf/domain/study-and-research-skills"/>
                  <skos:inScheme rdf:resource="https://data.ox.ac.uk/id/ox-rdf/concept-scheme"/>
               </skos:Concept>
            </skos:narrower>
            <skos:narrower>
               <skos:Concept rdf:about="https://data.ox.ac.uk/id/ox-rdf/descriptor/IL">
                  <skos:prefLabel>Interpersonal skills</skos:prefLabel>
                  <skos:notation rdf:datatype="https://data.ox.ac.uk/id/ox-rdf/notation">IL</skos:notation>
                  <skos:definition>How good are you at working with, managing, influencing, or leading others, as a team leader or member, supervisor, mentor or mentee?</skos:definition>
                  <skos:related rdf:resource="https://data.ox.ac.uk/id/ox-rdf/domain/teaching-and-academic-skills"/>
                  <skos:inScheme rdf:resource="https://data.ox.ac.uk/id/ox-rdf/concept-scheme"/>
               </skos:Concept>
            </skos:narrower>
            <skos:narrower>
               <skos:Concept rdf:about="https://data.ox.ac.uk/id/ox-rdf/descriptor/LS">
                  <skos:prefLabel>Laboratory skills</skos:prefLabel>
                  <skos:notation rdf:datatype="https://data.ox.ac.uk/id/ox-rdf/notation">LS</skos:notation>
                  <skos:definition>This includes knowledge and application: watch your step!</skos:definition>
                  <skos:related rdf:resource="https://data.ox.ac.uk/id/ox-rdf/domain/study-and-research-skills"/>
                  <skos:inScheme rdf:resource="https://data.ox.ac.uk/id/ox-rdf/concept-scheme"/>
               </skos:Concept>
            </skos:narrower>
            <skos:narrower>
               <skos:Concept rdf:about="https://data.ox.ac.uk/id/ox-rdf/descriptor/RF">
                  <skos:prefLabel>Research and financial management</skos:prefLabel>
                  <skos:notation rdf:datatype="https://data.ox.ac.uk/id/ox-rdf/notation">RF</skos:notation>
                  <skos:definition>This skill is all about the practice of managing projects: managing resources and finances; generating income; understanding risk; planning and delivering the end result, and so on.</skos:definition>
                  <skos:related rdf:resource="https://data.ox.ac.uk/id/ox-rdf/domain/study-and-research-skills"/>
                  <skos:inScheme rdf:resource="https://data.ox.ac.uk/id/ox-rdf/concept-scheme"/>
               </skos:Concept>
            </skos:narrower>
            <skos:narrower>
               <skos:Concept rdf:about="https://data.ox.ac.uk/id/ox-rdf/descriptor/HS">
                  <skos:prefLabel>Safety</skos:prefLabel>
                  <skos:notation rdf:datatype="https://data.ox.ac.uk/id/ox-rdf/notation">HS</skos:notation>
                  <skos:definition>Don't slip - record your knowledge and application of health and safety here.</skos:definition>
                  <skos:related rdf:resource="https://data.ox.ac.uk/id/ox-rdf/domain/study-and-research-skills"/>
                  <skos:inScheme rdf:resource="https://data.ox.ac.uk/id/ox-rdf/concept-scheme"/>
               </skos:Concept>
            </skos:narrower>
            <skos:narrower>
               <skos:Concept rdf:about="https://data.ox.ac.uk/id/ox-rdf/descriptor/CS">
                  <skos:prefLabel>Communication skills</skos:prefLabel>
                  <skos:notation rdf:datatype="https://data.ox.ac.uk/id/ox-rdf/notation">CS</skos:notation>
                  <skos:definition>Are you good at getting the message across to a broad range of people or publics, including students, and in a range of media (including social media)?</skos:definition>
                  <skos:related rdf:resource="https://data.ox.ac.uk/id/ox-rdf/domain/communication"/>
                  <skos:inScheme rdf:resource="https://data.ox.ac.uk/id/ox-rdf/concept-scheme"/>
               </skos:Concept>
            </skos:narrower>
            <skos:narrower>
               <skos:Concept rdf:about="https://data.ox.ac.uk/id/ox-rdf/descriptor/EE">
                  <skos:prefLabel>Enterprise and Entrepreneurship</skos:prefLabel>
                  <skos:notation rdf:datatype="https://data.ox.ac.uk/id/ox-rdf/notation">EE</skos:notation>
                  <skos:definition>Includes your skills in developing business ideas, influencing policy, society and culture in an entrepreneurial way, thinking globally, and so on.</skos:definition>
                  <skos:related rdf:resource="https://data.ox.ac.uk/id/ox-rdf/domain/communication"/>
                  <skos:inScheme rdf:resource="https://data.ox.ac.uk/id/ox-rdf/concept-scheme"/>
               </skos:Concept>
            </skos:narrower>
            <skos:narrower>
               <skos:Concept rdf:about="https://data.ox.ac.uk/id/ox-rdf/descriptor/PS">
                  <skos:prefLabel>Presentation skills</skos:prefLabel>
                  <skos:notation rdf:datatype="https://data.ox.ac.uk/id/ox-rdf/notation">PS</skos:notation>
                  <skos:definition>This includes all sorts of presenting, from teaching to pitching for investment - how is your knowledge of techniques and your self-confidence?</skos:definition>
                  <skos:related rdf:resource="https://data.ox.ac.uk/id/ox-rdf/domain/communication"/>
                  <skos:inScheme rdf:resource="https://data.ox.ac.uk/id/ox-rdf/concept-scheme"/>
               </skos:Concept>
            </skos:narrower>
            <skos:narrower>
               <skos:Concept rdf:about="https://data.ox.ac.uk/id/ox-rdf/descriptor/SC">
                  <skos:prefLabel>Seminars / Colloquia</skos:prefLabel>
                  <skos:notation rdf:datatype="https://data.ox.ac.uk/id/ox-rdf/notation">SC</skos:notation>
                  <skos:definition>This is about your performance in group learning or presenting situations - can you contribute in a valuable way, can you influence the group when you want to, or have you done some public engagement in this kind of setting?</skos:definition>
                  <skos:related rdf:resource="https://data.ox.ac.uk/id/ox-rdf/domain/communication"/>
                  <skos:inScheme rdf:resource="https://data.ox.ac.uk/id/ox-rdf/concept-scheme"/>
               </skos:Concept>
            </skos:narrower>
            <skos:narrower>
               <skos:Concept rdf:about="https://data.ox.ac.uk/id/ox-rdf/descriptor/TA">
                  <skos:prefLabel>Teaching &amp; Academic skills</skos:prefLabel>
                  <skos:notation rdf:datatype="https://data.ox.ac.uk/id/ox-rdf/notation">TA</skos:notation>
                  <skos:definition>Includes knowledge and application of pedagogy and of being an academic (a good academic citizen, if you will).</skos:definition>
                  <skos:related rdf:resource="https://data.ox.ac.uk/id/ox-rdf/domain/teaching-and-academic-skills"/>
                  <skos:inScheme rdf:resource="https://data.ox.ac.uk/id/ox-rdf/concept-scheme"/>
               </skos:Concept>
            </skos:narrower>
         </skos:Concept>
      </skos:hasTopConcept>
      <skos:hasTopConcept>
         <skos:Concept rdf:about="https://data.ox.ac.uk/id/ox-rdf/domain/top">
            <skos:prefLabel>Root skill domain</skos:prefLabel>
            <skos:narrower>
               <skos:Concept rdf:about="https://data.ox.ac.uk/id/ox-rdf/domain/study-and-research-skills">
                  <skos:prefLabel>Study and Research skills</skos:prefLabel>
               </skos:Concept>
            </skos:narrower>
            <skos:narrower>
               <skos:Concept rdf:about="https://data.ox.ac.uk/id/ox-rdf/domain/career-and-personal-development">
                  <skos:prefLabel>Career and Personal Development</skos:prefLabel>
               </skos:Concept>
            </skos:narrower>
            <skos:narrower>
               <skos:Concept rdf:about="https://data.ox.ac.uk/id/ox-rdf/domain/teaching-and-academic-skills">
                  <skos:prefLabel>Teaching and academic skills</skos:prefLabel>
               </skos:Concept>
            </skos:narrower>
            <skos:narrower>
               <skos:Concept rdf:about="https://data.ox.ac.uk/id/ox-rdf/domain/communication">
                  <skos:prefLabel>Communication</skos:prefLabel>
               </skos:Concept>
            </skos:narrower>
         </skos:Concept>
      </skos:hasTopConcept>
   </skos:ConceptScheme>
</rdf:RDF>